@prefix dbpedia-yago: <http://dbpedia.org/class/yago/> .
@prefix dbpedia: <http://dbpedia.org/resource/> .
@prefix iri: <http://data.openlinksw.com/oplweb/glossary-term/IRI#> .
@prefix uri: <http://data.openlinksw.com/oplweb/glossary-term/URI#> .
@prefix tuple: <http://data.openlinksw.com/oplweb/glossary-term/Tuple#> .
@prefix odbc: <http://data.openlinksw.com/oplweb/glossary-term/OpenDatabaseConnectivity#> .
@prefix jdbc: <http://data.openlinksw.com/oplweb/glossary-term/OpenDatabaseConnectivity#> .
@prefix tables: <http://data.openlinksw.com/oplweb/glossary-term/SQLRelation#> .
@prefix rdf-graphs: <http://data.openlinksw.com/oplweb/glossary-term/RDFRelation#> .
@prefix rdf-turtle: <http://data.openlinksw.com/oplweb/glossary-term/Turtle#> .
@prefix rdf-ntriples: <http://data.openlinksw.com/oplweb/glossary-term/NTriples#> .
@prefix rdf-xml: <http://data.openlinksw.com/oplweb/glossary-term/RDFXML#> .
@prefix json-ld: <http://data.openlinksw.com/oplweb/glossary-term/JSONLD#> .  
@prefix html-microdata: <http://data.openlinksw.com/oplweb/glossary-term/Microdata#> .
@prefix xhtml-rdfa: <http://data.openlinksw.com/oplweb/glossary-term/RDFa#> .
@prefix csv: <http://data.openlinksw.com/oplweb/glossary-term/CSV#> . 
@prefix sql-ddl: <http://data.openlinksw.com/oplweb/glossary-term/SQL#> . 
@prefix rdf-ddl: <http://data.openlinksw.com/oplweb/glossary-term/RDF#> .
@prefix owl-ddl: <http://data.openlinksw.com/oplweb/glossary-term/OWL#> .
@prefix spin-lang: <http://data.openlinksw.com/oplweb/glossary-term/SPINRulesVocab#> . 
@prefix rbac: <http://data.openlinksw.com/oplweb/glossary-term/RBAC#> .
@prefix abac: <http://data.openlinksw.com/oplweb/glossary-term/ABAC#> .
@prefix rdf-schema: <http://data.openlinksw.com/oplweb/glossary-term/RDFSchema#> .
@prefix sparql: <http://data.openlinksw.com/oplweb/glossary-term/SPARQL#> .
@prefix lubm: <http://swat.cse.lehigh.edu/projects/lubm/> . 
@prefix bsbm: <http://wifo5-03.informatik.uni-mannheim.de/bizer/berlinsparqlbenchmark/> .
@prefix hobbit-fct: <https://github.com/hobbit-project/faceted-benchmark#> .
@prefix ldbc: <http://ldbcouncil.org/> . 
@prefix ldbc-spb: <http://ldbcouncil.org/benchmarks/spb#> .
@prefix tpca: <http://www.tpc.org/tpca/default.asp#> .
@prefix tpcc: <http://www.tpc.org/tpcc/default.asp#> .
@prefix tpch: <http://www.tpc.org/tpch/default.asp#> .
@prefix cc:      <http://creativecommons.org/ns#> .
@prefix dbms-ontology: <http://www.openlinksw.com/ontology/dbms#> .
@prefix xsd: <http://www.w3.org/2001/XMLSchema#> .
@prefix owl: <http://www.w3.org/2002/07/owl#> . 
@prefix : <http://www.openlinksw.com/ontology/dbms#> .
@prefix source:      <http://www.openlinksw.com/data/turtle/dbms-ontology.ttl> .
@prefix sourceDAV:   <http://www.openlinksw.com/DAV/data/turtle/dbms-ontology.ttl> .

sourceDAV:
    a schema:CreativeWork ;
    schema:author <http://www.openlinksw.com/#this> ;
    xhv:license <http://creativecommons.org/licenses/by/4.0/deed.en_US> ;
    cc:attributionName "OpenLink Software" ;
    cc:attributionURL <http://www.openlinksw.com/dataspace/organization/openlink#this> ;
    schema:datePublished "2019-04-18T13:00:00-05:00"^^xsd:dateTime ;
    schema:dateCreated "2019-04-17T13:00:00-05:00"^^xsd:dateTime ;
    schema:dateModified "2019-04-18T15:00:00-05:00"^^xsd:dateTime ;
    schema:name  """OpenLink Database Ontology Document """ ;
    schema:description  """Document that describes an Ontology of terms associated with 
						   Database Management Systems (DBMS) genres. Terms in this ontology enable
						   structured descriptions of DBMS products.  
						 """^^xsd:string ;
    schema:keywords  """ODBC, ODBC Driver, JDBC, JDBC Driver, ADO.NET, ADO.NET Provider, OLE-DB, OLE-DB Provider, 
						UDA, Data Access, Data Access Driver, Data Access Middleware, Database, Database Management System, 
						DBMS, Relational Database Management System, RDBMS, Resource Description Framework, RDF, Relation,
						NoSQL, SQL, SPARQL.
		 			 """;
    owl:sameAs source: .


dbms-ontology:this a owl:Ontology ;
rdfs:label """OpenLink Database Management Systems Ontology"""^^xsd:string ;
rdfs:comment """Ontology that defines entity and relation types used to describe 
			  Database Management Systems software.
		   """@en ;
dcterms:created "2019-04-17T13:00:00-05:00"^^xsd:dateTime ;
schema:creator <http://www.openlinksw.com/#this> ;
dcterms:modified "2019-04-17T16:21:00-05:00"^^xsd:dateTime ;
owl:versionInfo "1.0.0"^^xsd:string ;
wdrs:describedby <> . 

## Classes

:DatabaseManagementSystem
rdfs:subClassOf schema:Application ;
rdfs:label "Database Management System" ;
skos:altLabel "DBMS" ;
rdfs:comment "A Software Application that provides Structured Data Definition and Manipulation functionality." ;
owl:equivalentClass dbpedia-yago:DatabaseManagementSystem106588785 ;
schema:maninEntityOfPage <https://docs.google.com/spreadsheets/d/1QHbPEsZqyNb6k0JB5j8vHkuI514c44mkNu-SaO8DekM/edit#gid=1757189899>,
	 					 <http://www.openlinksw.com/data/turtle/general/tabulated-data-comparison.ttl>,
						 <http://linkeddata.uriburner.com/describe/?url=https%3A%2F%2Fwww.openlinksw.com%2Fdata%2Fturtle%2Fgeneral%2Ftabulated-data-comparison.ttl%23content&graph=http%3A%2F%2Fwww.openlinksw.com%2Fdata%2Fturtle%2Fgeneral%2Ftabulated-data-comparison.ttl&distinct=1> ;
rdfs:isDefinedBy dbms-ontology:this . 

## Properties 

:supportsIdentifierType
a owl:ObjectProperty ;
rdfs:label "supportsIdentifierType" ;
rdfs:comment """Associates a Database Management System (DBMS) with supported Identifier Types. Examples include
              IRIs, URIs, and other""" ;
rdfs:domain :DatabaseManagementSystem ;
rdfs:range dbpedia-yago:Identifier107270601 ;
skos:related iri:this, uri:this ;
rdfs:isDefinedBy dbms-ontology:this . 

:identifierQuoteChar
a owl:ObjectProperty ;
rdfs:label "identifierQuoteChar" ;
rdfs:comment """Associates a Database Management System (DBMS) with supported Identifier Quotation character 
                for system artificat naming/identification (relations/tables, inferred-relations/views, stored procedures)
				e.g., double-quotes, single-quotes, less-than and greater-than characters""" ;
rdfs:domain :DatabaseManagementSystem ;
rdfs:range xsd:literal ;
skos:related iri:this, uri:this ;
rdfs:isDefinedBy dbms-ontology:this . 


:relationsModeledAs
a owl:ObjectProperty ;
rdfs:label "relationsModeledAs" ;
rdfs:comment """Associates a Database Management System (DBMS) with how it models Entity Relationship Types (Relations)""" ;
rdfs:domain :DatabaseManagementSystem ;
rdfs:range dbpedia-yago:Sequence108459252 ;
skos:related tables:this, rdf-graphs:this, dbpedia:Directed_graph ;
rdfs:isDefinedBy dbms-ontology:this . 


:relationStructure
a owl:ObjectProperty ;
rdfs:label "relationStructure" ;
rdfs:comment """Associates a Database Management System (DBMS) with how it Entity Relationship Types (Relations) 
				are structured e.g., N-Tuples, 3-Tuples etc.
			 """ ;
rdfs:domain :DatabaseManagementSystem ;
rdfs:range dbpedia-yago:DataStructure105728493 ;
skos:related dbpedia:Semantic_triple, dbpedia:Tuple, tuple:this ;
rdfs:isDefinedBy dbms-ontology:this . 

:relationPartitioning
a owl:ObjectProperty ;
rdfs:label "relationPartitioning" ;
rdfs:comment """Associates a Database Management System (DBMS) with how it partitions relations
                for unambiguous identification using namespacing. For example: catalog.schema.relation,
				database.schema.relation, schema.relation, urn:xyz:data, http://example.com/entity/,
				or http://example.com/entity#this etc.
			 """ ;
rdfs:domain :DatabaseManagementSystem ;
rdfs:range xsd:literal ;
skos:related dbpedia:Semantic_triple, dbpedia:Tuple, tuple:this ;
rdfs:isDefinedBy dbms-ontology:this . 


:tupleNotation
a owl:ObjectProperty ;
rdfs:label "tupleNotation" ;
rdfs:comment """Associates a Database Management System (DBMS) with the supported notations for
				representing N-Tuples, 3-Tuples etc.
			 """ ;
rdfs:domain :DatabaseManagementSystem ;
rdfs:range dbpedia-yago:Notation106808493 ;
skos:related rdf-turtle:this, rdf-ntriples:this, rdf-xml:this, json-ld:this, html-microdata:this,
			 xhtml-rdfa:this, csv:this, tuple:this ;
rdfs:isDefinedBy dbms-ontology:this . 


:declarativeDataDefinitionLang
a owl:ObjectProperty ;
rdfs:label "declarativeDataDefinitionLang" ;
skos:altLabel "DDL" ;
rdfs:comment """Associates a Database Management System (DBMS) with supported declarative 
				Data Definition Languages.
			 """ ;
rdfs:domain :DatabaseManagementSystem ;
rdfs:range dbpedia-yago:WikicatDataModelingLanguages ;
skos:related rdf-ddl:this, owl-ddl:this, sql-ddl:this ;
rdfs:isDefinedBy dbms-ontology:this . 


:declarativeDataManipulationLang
a owl:ObjectProperty ;
rdfs:label "declarativeDataManipulationLang" ;
skos:altLabel "DML" ;
rdfs:comment """Associates a Database Management System (DBMS) with supported declarative 
				Data Manipulation Languages.
			 """ ;
rdfs:domain :DatabaseManagementSystem ;
rdfs:range dbpedia-yago:WikicatQueryLanguages ;
skos:related sparql:this, sql-ddl:this, rdf-schema:this, owl-ddl:this, rdf-ddl:this ;
rdfs:isDefinedBy dbms-ontology:this . 

:declarativeReasoningLang
a owl:ObjectProperty ;
rdfs:label "declarativeReasoningLang" ;
rdfs:comment """Associates a Database Management System (DBMS) with supported declarative 
				Reasoning & Inference Languages.
			 """ ;
rdfs:domain :DatabaseManagementSystem ;
rdfs:range dbpedia-yago:ArtificialLanguage106894544, dbpedia-yago:WikicatQueryLanguages ;
skos:related spin-lang:this, sparql:this, sql-ddl:this ;
rdfs:isDefinedBy dbms-ontology:this . 


:dataAccessAPI
a owl:ObjectProperty ;
rdfs:label "dataAccessAPI" ;
rdfs:altLabel "Data Access API" ;
rdfs:comment """Associates a Database Management System (DBMS) with supported Data
				Access Programming Interfaces e.g., ODBC, JDBC, ADO.NET, OLE-DB, 
				XMLA, HTTP etc.
			 """ ;
rdfs:domain :DatabaseManagementSystem ;
rdfs:range dbpedia-yago:WikicatComputerLibraries ;
skos:related odbc:this, jdbc:this ;
rdfs:isDefinedBy dbms-ontology:this . 


:transactionSemantics
a owl:ObjectProperty ;
rdfs:label "transactionSemantics" ;
skos:altLabel "ACID" ;
rdfs:comment """Associates a Database Management System (DBMS) with supported Transaction Semantics e.g.,
                Atomicity (A), Consistency (C), Isolation (I), and Durability (D).
			 """ ;
rdfs:domain :DatabaseManagementSystem ;
rdfs:range skos:Concept ;
skos:related dbpedia:Transaction_processing, dbpedia:ACID ;
rdfs:isDefinedBy dbms-ontology:this . 

:dataAccessControl
a owl:ObjectProperty ;
rdfs:label "dataAccessControl" ;
skos:altLabel "Data Security" ;
rdfs:comment """Associates a Database Management System (DBMS) with supported modalities
				for controlling access to data e.g., Role-based Access Control (RBAC) or 
				Attributed-based Access Control (ABAC).
			 """ ;
rdfs:domain :DatabaseManagementSystem ;
rdfs:range dbpedia-yago:Identifier107270601 ;
skos:related rbac:this, abac:this ;
rdfs:isDefinedBy dbms-ontology:this . 


:benchmarkStandards
a owl:ObjectProperty ;
rdfs:label "benchmarkStandards" ;
skos:altLabel "Industry Standard Performance Benchmarks" ;
rdfs:comment """Associates a Database Management System (DBMS) with supported industry standard
				benchmarks e.g., TPC-A, TPC-D, TPC-H, LDBC, LUBM, Berlin SPARQL Benchmark etc..
			 """ ;
rdfs:domain :DatabaseManagementSystem ;
rdfs:range dbpedia-yago:Identifier107270601 ;
skos:related lubm:this, bsbm:this, hobbit-fct:this, ldbc:this, ldbc-spb:this, tpca:this, tpcc:this,
			 tpch:this ;
rdfs:isDefinedBy dbms-ontology:this . 
