## LinkedIn Tags
@prefix LinkedInTagGraphDatabases:    <https://www.linkedin.com/feed/topic/?keywords=%23GraphDatabase#> .
@prefix LinkedInTagGraphDatabase:     <https://www.linkedin.com/feed/topic/?keywords=%23GraphDatabases#> .
@prefix LinkedInTagGraphDB:           <https://www.linkedin.com/feed/topic/?keywords=%23GraphDB#> .
@prefix LinkedInTagDocumentDatabases: <https://www.linkedin.com/feed/topic/?keywords=%23DocumentDatabase#> .
@prefix LinkedInTagDocumentDatabase:  <https://www.linkedin.com/feed/topic/?keywords=%23DocumentDatabases#> .
@prefix LinkedInTagDocumentDB:        <https://www.linkedin.com/feed/topic/?keywords=%23DocumentDB#> .
@prefix LinkedInTagLinkedData:        <https://www.linkedin.com/feed/topic/?keywords=%23LinkedData#> .
@prefix LinkedInTagLinkedData:        <https://www.linkedin.com/feed/topic/?keywords=%23LinkedData#> .
@prefix LinkedInTagSemanticWeb:       <https://www.linkedin.com/feed/topic/?keywords=%23SemanticWeb#> .
@prefix LinkedInTagRDBMS:             <https://www.linkedin.com/feed/topic/?keywords=%23RDBMS#> .
@prefix LinkedInTagKnowledgeGraph:    <https://www.linkedin.com/feed/topic/?keywords=%23KnowledgeGraph#> .

## Twitter Tags

@prefix TwitterTagGraphDatabases:     <https://twitter.com/hashtag/GraphDatabases#> .
@prefix TwitterTagGraphDatabase:      <https://twitter.com/hashtag/GraphDatabase#> .
@prefix TwitterTagGraphDB:            <https://twitter.com/hashtag/GraphDB#> .
@prefix TwitterTagDocumentDatabases:  <https://twitter.com/hashtag/DocumentDatabases#> .
@prefix TwitterTagDocumentDatabase:   <https://twitter.com/hashtag/DocumentDatabase#> .
@prefix TwitterTagDocumentDB:         <https://twitter.com/hashtag/DocumentDB#> .
@prefix TwitterTagRDBMS:              <https://twitter.com/hashtag/RDBMS#> .
@prefix TwitterTagKnowledgeGraph:     <https://twitter.com/hashtag/KnowledgeGraph#> .

## Facebook Tags

@prefix FacebookTagGraphDatabase:     <https://www.facebook.com/hashtag/GraphDatabase#> .
@prefix FacebookTagGraphDatabases:    <https://www.facebook.com/hashtag/GraphDatabases#> .
@prefix FacebookTagGraphDB:           <https://www.facebook.com/hashtag/GraphDB#> .
@prefix FacebookTagDocumentDatabase:  <https://www.facebook.com/hashtag/DocumentDatabase#> .
@prefix FacebookTagDocumentDatabases: <https://www.facebook.com/hashtag/DocumentDatabases#> .
@prefix FacebookTagDocumentDB:        <https://www.facebook.com/hashtag/DocumentDB#> .
@prefix FacebookTagLinkedData:        <https://www.facebook.com/hashtag/LinkedData#> .
@prefix FacebookTagSemanticWeb:       <https://www.facebook.com/hashtag/SemanticWeb#> .
@prefix FacebookTagRDBMS:             <https://www.facebook.com/hashtag/RDBMS#> .
@prefix FacebookTagRDBMS:             <https://www.facebook.com/hashtag/KnowledgeGraph#> .
@prefix FacebookTagKnowledgeGraph:    <https://www.facebook.com/hashtag/KnowledgeGraph#> .

## Others

@prefix                : <http://www.openlinksw.com/ontology/dbms-app-ontology#> .
@prefix            abac: <http://data.openlinksw.com/oplweb/glossary-term/ABAC#> .
@prefix            bsbm: <http://wifo5-03.informatik.uni-mannheim.de/bizer/berlinsparqlbenchmark/> .
@prefix              cc: <http://creativecommons.org/ns#> .
@prefix             csv: <http://data.openlinksw.com/oplweb/glossary-term/CSV#> .
@prefix        database: <http://data.openlinksw.com/oplweb/glossary-term/Database#> .
@prefix    dbpedia-yago: <http://dbpedia.org/class/yago/> .
@prefix         dbpedia: <http://dbpedia.org/resource/> .
@prefix         dcterms: <http://purl.org/dc/terms/> .
@prefix      hobbit-fct: <https://github.com/hobbit-project/faceted-benchmark#> .
@prefix  html-microdata: <http://data.openlinksw.com/oplweb/glossary-term/Microdata#> .
@prefix             iri: <http://data.openlinksw.com/oplweb/glossary-term/IRI#> .
@prefix            jdbc: <http://data.openlinksw.com/oplweb/glossary-term/OpenDatabaseConnectivity#> .
@prefix         json-ld: <http://data.openlinksw.com/oplweb/glossary-term/JSONLD#> .
@prefix        ldbc-spb: <http://ldbcouncil.org/benchmarks/spb#> .
@prefix            ldbc: <http://ldbcouncil.org/> .
@prefix            lubm: <http://swat.cse.lehigh.edu/projects/lubm/> .
@prefix            odbc: <http://data.openlinksw.com/oplweb/glossary-term/OpenDatabaseConnectivity#> .
@prefix         owl-ddl: <http://data.openlinksw.com/oplweb/glossary-term/OWL#> .
@prefix             owl: <http://www.w3.org/2002/07/owl#> .
@prefix            rbac: <http://data.openlinksw.com/oplweb/glossary-term/RBAC#> .
@prefix         rdf-ddl: <http://data.openlinksw.com/oplweb/glossary-term/RDF#> .
@prefix      rdf-graphs: <http://data.openlinksw.com/oplweb/glossary-term/RDFRelation#> .
@prefix    rdf-ntriples: <http://data.openlinksw.com/oplweb/glossary-term/NTriples#> .
@prefix    rdf-relation: <http://data.openlinksw.com/oplweb/glossary-term/RDFRelation#> .
@prefix      rdf-schema: <http://data.openlinksw.com/oplweb/glossary-term/RDFSchema#> .
@prefix      rdf-turtle: <http://data.openlinksw.com/oplweb/glossary-term/Turtle#> .
@prefix         rdf-xml: <http://data.openlinksw.com/oplweb/glossary-term/RDFXML#> .
@prefix            rdfs: <http://www.w3.org/2000/01/rdf-schema#> .
@prefix          schema: <http://schema.org/> .
@prefix            skos: <http://www.w3.org/2004/02/skos/core#> .
@prefix          source: <http://www.openlinksw.com/ontology/dbms-app-ontology#> .
@prefix       sourceDAV: <http://www.openlinksw.com/DAV/data/turtle/dbms-app-ontology.ttl> .
@prefix sparql-protocol: <http://data.openlinksw.com/oplweb/glossary-term/SPARQLProtocol#> .
@prefix          sparql: <http://data.openlinksw.com/oplweb/glossary-term/SPARQL#> .
@prefix       spin-lang: <http://data.openlinksw.com/oplweb/glossary-term/SPINRulesVocab#> .
@prefix         sql-ddl: <http://data.openlinksw.com/oplweb/glossary-term/SQL#> .
@prefix    sql-relation: <http://data.openlinksw.com/oplweb/glossary-term/SQLRelation#> .
@prefix          tables: <http://data.openlinksw.com/oplweb/glossary-term/SQLRelation#> .
@prefix            tpca: <http://www.tpc.org/tpca/default.asp#> .
@prefix            tpcc: <http://www.tpc.org/tpcc/default.asp#> .
@prefix            tpch: <http://www.tpc.org/tpch/default.asp#> .
@prefix           tuple: <http://data.openlinksw.com/oplweb/glossary-term/Tuple#> .
@prefix             uri: <http://data.openlinksw.com/oplweb/glossary-term/URI#> .
@prefix        virtuoso: <http://data.openlinksw.com/oplweb/product/Virtuoso#> .
@prefix            wdrs: <http://www.w3.org/2007/05/powder-s#> .
@prefix      xhtml-rdfa: <http://data.openlinksw.com/oplweb/glossary-term/RDFa#> .
@prefix             xhv: <http://www.w3.org/1999/xhtml/vocab#> .
@prefix             xsd: <http://www.w3.org/2001/XMLSchema#> .
# @prefix dbms-ontology:   <http://www.openlinksw.com/ontology/dbms#> .

sourceDAV:
    a                    schema:CreativeWork ;
    schema:author        <http://www.openlinksw.com/#this> ;
    xhv:license          <http://creativecommons.org/licenses/by/4.0/deed.en_US> ;
    cc:attributionName   "OpenLink Software"@en ;
    cc:attributionURL    <http://www.openlinksw.com/dataspace/organization/openlink#this> ;
    schema:datePublished "2019-04-18T13:00:00-05:00"^^xsd:dateTime ;
    schema:dateCreated   "2019-04-17T13:00:00-05:00"^^xsd:dateTime ;
    dcterms:modified     "2019-06-11T17:00:00-04:00"^^xsd:dateTime ;
    schema:name          """OpenLink Database Management System Ontology Document"""@en ;
    schema:description   """Document that describes an Ontology of terms associated with
                            Database Management Systems (DBMS) genres. Terms in this ontology enable
                            structured descriptions of DBMS products.
                         """@en ;
    schema:keywords      "ODBC" ,
                         "ODBC Driver"@en ,
                         "JDBC" ,
                         "JDBC Driver"@en ,
                         "ADO.NET" ,
                         "ADO.NET Provider"@en ,
                         "OLE DB" ,
                         "OLE DB Provider"@en ,
                         "UDA" ,
                         "Data Access"@en ,
                         "Data Access Driver"@en ,
                         "Data Access Middleware"@en ,
                         "Database"@en ,
                         "Database Management System"@en ,
                         "DBMS" ,
                         "Relational Database Management System"@en ,
                         "RDBMS" ,
                         "Resource Description Framework"@en ,
                         "RDF" ,
                         "Relation"@en ,
                         "NoSQL"@en ,
                         "SQL" ,
                         "SPARQL" ;
    schema:mainEnity : ;
    owl:sameAs source: .

: 
    a               owl:Ontology ;
    dcterms:title   """OpenLink Database Management Systems Ontology"""@en ;
    rdfs:label      """OpenLink Database Management Systems Ontology"""@en ;
    rdfs:comment    """Ontology that defines entity and relation types used to describe
                       Database Management Systems software.
                    """@en ;
    dcterms:created  "2019-04-17T13:00:00-05:00"^^xsd:dateTime ;
    schema:creator   <http://www.openlinksw.com/#this> ;
    dcterms:modified "2019-06-11T17:00:00-04:00"^^xsd:dateTime ;
    owl:versionInfo  "1.0.0"^^xsd:string ;
    wdrs:describedby <> .

## Classes

:DatabaseManagementSystem
    rdfs:subClassOf          schema:Application ;
    rdfs:label               "Database Management System"@en ;
    skos:altLabel            "DBMS" ;
    rdfs:comment             "A Software Application that provides Structured Data Definition and Manipulation functionality."@en ;
    owl:equivalentClass      dbpedia-yago:DatabaseManagementSystem106588785 ;
    skos:related             LinkedInTagGraphDatabases:this , 
                             LinkedInTagDocumentDatabase:this , 
                             LinkedInTagDocumentDB:this ,
                             LinkedInTagRDBMS:this , 
                             TwitterTagGraphDatabases:this , 
                             TwitterTagDocumentDatabase:this ,
                             TwitterTagDocumentDB:this , 
                             TwitterTagRDBMS:this , 
                             FacebookTagGraphDatabases:this ,
                             FacebookTagDocumentDatabase:this , 
                             FacebookTagDocumentDB:this , 
                             FacebookTagRDBMS:this ;
    schema:maninEntityOfPage <https://docs.google.com/spreadsheets/d/1QHbPEsZqyNb6k0JB5j8vHkuI514c44mkNu-SaO8DekM/edit#gid=1757189899> ,
                             <http://www.openlinksw.com/data/turtle/general/tabulated-data-comparison.ttl> ,
                             <http://linkeddata.uriburner.com/describe/?url=https%3A%2F%2Fwww.openlinksw.com%2Fdata%2Fturtle%2Fgeneral%2Ftabulated-data-comparison.ttl%23content&graph=http%3A%2F%2Fwww.openlinksw.com%2Fdata%2Fturtle%2Fgeneral%2Ftabulated-data-comparison.ttl&distinct=1> ;
    rdfs:isDefinedBy : .

## External Classes

dbpedia-yago:Identifier107270601 
    rdfs:label "Class: Identifier"@en .
dbpedia-yago:Sequence108459252 
    rdfs:label "Class: Sequence"@en .
dbpedia-yago:WikicatComputerLibraries 
    rdfs:label "Class: Computer Library"@en .
dbpedia-yago:ArtificialLanguage106894544 
    rdfs:label "Class: Artificial Language"@en .
dbpedia-yago:WikicatQueryLanguages 
    rdfs:label "Class: Query Language"@en .
dbpedia-yago:WikicatDataModelingLanguages 
    rdfs:label "Class: Modeling Language"@en .
dbpedia-yago:Notation106808493 
    rdfs:label "Class: Notation"@en .
dbpedia-yago:DataStructure105728493 
    rdfs:label "Class: Data Structure"@en .
dbpedia-yago:DatabaseManagementSystem106588785 
    rdfs:label "Class: Database Management System"@en .

## Properties

:supportsIdentifierType
    a                owl:ObjectProperty ;
    rdfs:label       "supportsIdentifierType"@en ;
    rdfs:comment     """Associates a Database Management System (DBMS) with supported Identifier Types. 
                        Examples include IRIs, URIs, and others.
                     """@en ;
    rdfs:domain      :DatabaseManagementSystem ;
    rdfs:range       dbpedia-yago:Identifier107270601 ;
    skos:related     iri:this, uri:this ;
    rdfs:isDefinedBy : .

:identifierQuoteChar
    a                owl:ObjectProperty ;
    rdfs:label       "identifierQuoteChar"@en ;
    rdfs:comment     """Associates a Database Management System (DBMS) with supported Identifier 
                        Quotation character for system artifact naming/identification (relations/tables, 
                        inferred-relations/views, stored procedures), e.g., double-quote, single-quote, 
                        less-than, and greater-than characters.
                     """@en ;
    rdfs:domain      :DatabaseManagementSystem ;
    rdfs:range       xsd:literal ;
    skos:related     iri:this, uri:this ;
    rdfs:isDefinedBy : .

:relationsModeledAs
    a                owl:ObjectProperty ;
    rdfs:label       "relationsModeledAs"@en ;
    rdfs:comment     """Associates a Database Management System (DBMS) with how its Entity Relationship 
                        Types (Relations) are modeled, e.g., Tables, Graphs, Trees, Hybrid, etc.
                     """@en ;
    rdfs:domain      :DatabaseManagementSystem ;
    rdfs:range       dbpedia-yago:Sequence108459252 ;
    skos:related     tables:this , 
                     rdf-graphs:this , 
                     dbpedia:Directed_graph ;
    rdfs:isDefinedBy : .

:relationStructure
    a                owl:ObjectProperty ;
    rdfs:label       "relationStructure"@en ;
    rdfs:comment     """Associates a Database Management System (DBMS) with how its Entity Relationship 
                        Types (Relations) are structured, e.g., N-Tuples, 3-Tuples, Key-Value Pairs, etc.
                     """@en ;
    rdfs:domain      :DatabaseManagementSystem ;
    rdfs:range       dbpedia-yago:DataStructure105728493 ;
    skos:related     dbpedia:Semantic_triple , 
                     dbpedia:Tuple , 
                     tuple:this ;
    rdfs:isDefinedBy : .

:relationPartitioning
    a                owl:ObjectProperty ;
    rdfs:label       "relationPartitioning"@en ;
    rdfs:comment     """Associates a Database Management System (DBMS) with how its relations are partitioned
                        for unambiguous identification using namespaces. For example: catalog.schema.relation,
                        database.schema.relation, schema.relation, urn:xyz:data, http://example.com/entity/,
                        http://example.com/entity#this, etc.
                     """@en ;
    rdfs:domain      :DatabaseManagementSystem ;
    rdfs:range       xsd:literal ;
    skos:related     dbpedia:Semantic_triple , 
                     dbpedia:Tuple , 
                     tuple:this ;
    rdfs:isDefinedBy : .

:tupleNotation
    a                owl:ObjectProperty ;
    rdfs:label       "tupleNotation"@en ;
    rdfs:comment     """Associates a Database Management System (DBMS) with the notations it supports for
                        representing N-Tuples, 3-Tuples, etc.
                     """@en ;
    rdfs:domain      :DatabaseManagementSystem ;
    rdfs:range       dbpedia-yago:Notation106808493 ;
    skos:related     rdf-turtle:this , 
                     rdf-ntriples:this , 
                     rdf-xml:this , 
                     json-ld:this , 
                     html-microdata:this ,
                     xhtml-rdfa:this , 
                     csv:this, 
                     tuple:this ;
    rdfs:isDefinedBy : .

:declarativeDataDefinitionLang
    a                owl:ObjectProperty ;
    rdfs:label       "declarativeDataDefinitionLang"@en ;
    skos:altLabel    "DDL" ;
    rdfs:comment     """Associates a Database Management System (DBMS) with the declarative
                        Data Definition Languages it supports.
                     """@en ;
    rdfs:domain      :DatabaseManagementSystem ;
    rdfs:range       dbpedia-yago:WikicatDataModelingLanguages ;
    skos:related     rdf-ddl:this , 
                     owl-ddl:this , 
                     sql-ddl:this ;
    rdfs:isDefinedBy : .

:declarativeDataManipulationLang
    a                owl:ObjectProperty ;
    rdfs:label       "declarativeDataManipulationLang"@en ;
    skos:altLabel    "DML" ;
    rdfs:comment     """Associates a Database Management System (DBMS) with the declarative
                       Data Manipulation Languages it supports.
                     """@en ;
    rdfs:domain      :DatabaseManagementSystem ;
    rdfs:range       dbpedia-yago:WikicatQueryLanguages ;
    skos:related     sparql:this , 
                     sql-ddl:this , 
                     rdf-schema:this , 
                     owl-ddl:this , 
                     rdf-ddl:this ;
    rdfs:isDefinedBy : .

:declarativeReasoningLang
    a                owl:ObjectProperty ;
    rdfs:label       "declarativeReasoningLang"@en ;
    rdfs:comment     """Associates a Database Management System (DBMS) with the declarative
                        Reasoning & Inference Languages it supports.
                     """@en ;
    rdfs:domain      :DatabaseManagementSystem ;
    rdfs:range       dbpedia-yago:ArtificialLanguage106894544, dbpedia-yago:WikicatQueryLanguages ;
    skos:related     spin-lang:this , 
                     sparql:this , 
                     sql-ddl:this ;
    rdfs:isDefinedBy : .

:dataAccessAPI
    a                owl:ObjectProperty ;
    rdfs:label       "dataAccessAPI"@en ;
    rdfs:altLabel    "Data Access API"@en ;
    rdfs:comment     """Associates a Database Management System (DBMS) with the Data
                        Access Programming Interfaces it supports, e.g., ODBC, JDBC, 
                        ADO.NET, OLE DB, XMLA, HTTP, etc.
                     """@en ;
    rdfs:domain      :DatabaseManagementSystem ;
    rdfs:range       dbpedia-yago:WikicatComputerLibraries ;
    skos:related     odbc:this , 
                     jdbc:this ;
    rdfs:isDefinedBy : .

:transactionSemantics
    a                owl:ObjectProperty ;
    rdfs:label       "transactionSemantics"@en ;
    skos:altLabel    "ACID" ;
    rdfs:comment     """Associates a Database Management System (DBMS) with the Transaction Semantics it 
                        supports, e.g., Atomicity (A), Consistency (C), Isolation (I), and/or Durability (D).
                     """@en ;
    rdfs:domain      :DatabaseManagementSystem ;
    rdfs:range       skos:Concept ;
    skos:related     dbpedia:Transaction_processing , 
                     dbpedia:ACID ;
    rdfs:isDefinedBy : .

:dataAccessControl
    a                owl:ObjectProperty ;
    rdfs:label       "dataAccessControl"@en ;
    skos:altLabel    "Data Security"@en ;
    rdfs:comment     """Associates a Database Management System (DBMS) with the modalities it supports
                        for controlling access to data, e.g., Role-based Access Control (RBAC) or
                        Attributed-based Access Control (ABAC).
                     """@en ;
    rdfs:domain      :DatabaseManagementSystem ;
    rdfs:range       dbpedia-yago:Identifier107270601 ;
    skos:related     rbac:this , 
                     abac:this ;
    rdfs:isDefinedBy : .

:benchmarkStandards
    a                owl:ObjectProperty ;
    rdfs:label       "benchmarkStandards"@en ;
    skos:altLabel    "Industry Standard Performance Benchmarks"@en ;
    rdfs:comment     """Associates a Database Management System (DBMS) with the industry standard
                        benchmarks it supports, e.g., TPC-A, TPC-D, TPC-H, LDBC, LUBM, Berlin 
                        SPARQL Benchmark, etc.
                     """@en ;
    rdfs:domain      :DatabaseManagementSystem ;
    rdfs:range       dbpedia-yago:Identifier107270601 ;
    skos:related     lubm:this , 
                     bsbm:this , 
                     hobbit-fct:this , 
                     ldbc:this , 
                     ldbc-spb:this , 
                     tpca:this , 
                     tpcc:this ,
                     tpch:this ;
    rdfs:isDefinedBy : .
